\documentclass[12pt,a4paper]{report}
\usepackage[T1]{fontenc}
\usepackage[utf8]{inputenc}
\usepackage{charter}
\usepackage{ngerman} \usepackage[left=2cm,right=2cm,top=2cm,bottom=2cm]{geometry}
\usepackage{amsmath}

\begin{document}
	\noindent
	\Large
	S. 161 Nr. 1b,c,d
	\large
	\paragraph{1b)}
	\begin{align*}
		\int_{0}^{2} (5x \cdot e^x) dx \\
		u = 5x;\ v = e^x; \\
		u' = 5;\ v' = e^x; \\
		\int_{0}^{2} (5x \cdot e^x)dx = \Bigl[5x \cdot e^x\Bigl]_{0}^{2} - \int_{0}^{2} (5 \cdot e^x) dx \\
		\Bigl[5x \cdot e^x - 5 \cdot e^x\Bigl]_{0}^{2} \\
		(5 \cdot 2 \cdot e^2 - 5 \cdot e^2) -
		(5 \cdot 0 \cdot e^0 - 5 \cdot e^0) \\
		(10e^2 - 5e^2) + 5 \\
		5e^2 + 5
	\end{align*}
	\paragraph{1c)}
	\begin{align*}
		\int_{0}^{1} (x \cdot e^{2x}) dx \\
		u = x;\ v = \frac{1}{2}e^{2x} \\
		u' = 1;\ v' = e^{2x} \\
		\int_{0}^{1} (x \cdot e^{2x})dx = \Bigl[x \cdot \frac{1}{2}e^{2x}\Bigl]_{0}^{1} - \int_{0}^{1} (1 \cdot \frac{1}{2}e^{2x}) \\
		\Bigl[x \cdot \frac{1}{2}e^{2x} - \frac{1}{4}e^{2x}\Bigl]_{0}^{1} \\
		(x \cdot \frac{1}{2}e^{2x} - \frac{1}{4}e^{2x}) - (x \cdot \frac{1}{2}e^{2x} - \frac{1}{4}e^{2x}) \\
		(\frac{1}{2}e^{2} - \frac{1}{4}e^{2}) - (0 \cdot \frac{1}{2}e^{0} - \frac{1}{4}e^{0}) \\
		\frac{1}{4}e^{2} + \frac{1}{4}
	\end{align*}
	\paragraph{1d)}
	\begin{align*}
		\int_{0}^{0.5}(4x \cdot e^{2x + 2}) dx \\
		u = 4x;\ v' = e^{2x + 2}; \\
		u' = 4;\ v = \frac{1}{2}e^{2x+2} \\
		\int_{0}^{0.5} (4x \cdot e^{2x+2})dx = \Bigl[4x \cdot \frac{1}{2}e^{2x+2}\Bigl]_{0}^{0.5} - \int_{0.5}^{0} (4 \cdot \frac{1}{2}e^{2x +2}) \\
		\Bigl[4x \cdot \frac{1}{2}e^{2x+2} - e^{2x+2}\Bigl] \\
		(2 \cdot \frac{1}{2}e^{1+2} - e^{1+2}) - (0 \cdot \frac{1}{2}e^{0+2} - e^{0+2}) \\	
		(e^{3} - e^{3}) + (e^{2}) \\
		e^2
	\end{align*}
\end{document}